\begin{problem}
    This problem introduces a simple meteorological model, more complicated versions of which have been proposed in the meteorological literature. Consider a sequence of days and let $R_i$ denote the event that it rains on day $i$. Suppose that $P(R_i \mid R_{i-1}) = \alpha$ and $P(R_i^c \mid R_{i-1}^c) = \beta$. Suppose further that only today's weather is relevant to predicting tomorrow's; that is $P(R_i \mid R_{i-1} \cap R_{i-2} \cap \dots \cap R_0) = P(R_i \mid R_{i-1})$.\\
    (a) If the probability of rain today is $p$, what is the probability of rain tomorrow?\\
    (b) What is the probability of rain the day after tomorrow?\\
    (c) What is the probability of rain $n$ days from now? What happens as $n$ approaches infinity?
    \end{problem}
    
    (a) Note that $R_{i-1}$ and $R_{i-1}^c$ union to the entire probability space. Therefore we can use the law of total probability to write
    \[
    P(R_i) = P(R_i \mid R_{i-1})P(R_{i-1}) + P(R_i \mid R_{i-1}^c)P(R_{i-1}^c) = \alpha p + (1 - \beta)(1 - p) = p(\alpha + \beta - 1) + (1 - \beta).
    \]
    
    (b) To find $P(R_{i+1})$ we use the same method as in part (a), but with $p$ replaced with $P(R_i)$. Thus
    \[
    P(R_{i+1}) = P(R_i)(\alpha + \beta - 1) + (1 - \beta) = (\alpha + \beta - 1)^2 p + (1 - \beta)(\alpha + \beta).
    \]
    
    (c) Let $x = (\alpha + \beta - 1)$ and $y = (1 - \beta)$. We are searching for $a_n$ such that $a_{n+1} = xa_n + y$ and $a_0 = p$. Let
    \[
    a_n = x^n p + y \frac{x^n - 1}{x - 1} = (\alpha + \beta - 1)^n p + (1 - \beta) \frac{(\alpha + \beta - 1)^n - 1}{\alpha + \beta - 2}.
    \]
    It's clear that $a_0 = p$. On the other hand,
    \begin{align*}
    a_{n+1}
    &= x^{n+1}p + y \frac{x^{n+1} - 1}{x-1}\\
    &= x^{n+1}p + y \frac{(x^{n+1} - x) + (x - 1)}{x-1}\\
    &= x^{n+1}p + y \left ( \frac{x^{n+1} - x}{x-1} + 1 \right )\\
    &= x \left ( x^n p + y \frac{x^n - 1}{x-1} \right ) + y\\
    &= x a_n + y
    \end{align*}
    so this fits our required relation. Note that $|x| = |\alpha + \beta - 1| < 1$ so $\lim_{n \rightarrow \infty} x^n = 0$ and
    \[
    \lim_{n \rightarrow \infty} a_n = \frac{-y}{x-1} = \frac{\beta - 1}{\alpha + \beta -2}.
    \]